# 2. Position and Orientation of Bodies

## 2.2 Matrix Algebra and Multivariable Calculus

- Lagrange Multiplier Theorem: If $\boldsymbol{x}^T\boldsymbol{c}=0$ for all $\boldsymbol{x}$ that satisfy $\boldsymbol{Bx}=\boldsymbol{0}$ then there exists a $\boldsymbol{\lambda}$ of Lagrange multipliers such that $\boldsymbol{c}+\boldsymbol{B}^T\boldsymbol{\lambda}=\boldsymbol{0}$

## 2.4 Position and Orientation of a Body in Space

### Identities Involving the Orientation Transformation Matrix

$$
\widetilde{\mathbf{s}}\mathbf{v}=\mathbf{A}\left(\widetilde{\mathbf{s}}^\prime\mathbf{v}^\prime\right)\\
\mathbf{v}=\mathbf{A}\mathbf{v}^\prime,\widetilde{\mathbf{s}}\left(\mathbf{A}\mathbf{v}^\prime\right)=\left(\widetilde{\mathbf{s}}\mathbf{A}\right)\mathbf{v}^\prime=\left(\mathbf{A}\widetilde{\mathbf{s}}^\prime\right)\mathbf{v}^\prime\\
\text{for arbitrary vectors }\mathbf{v}^\prime,\widetilde{\mathbf{s}}\mathbf{A}=\mathbf{A}\widetilde{\mathbf{s}}^\prime\\
\widetilde{\mathbf{s}}=\mathbf{A}\widetilde{\mathbf{s}}^\prime\mathbf{A}^\mathrm{T}
$$

### Velocity, Acceleration, Angular Velocity, and Angular Acceleration

$$
\mathbf{r}^\mathrm{P}=\mathbf{r}+\mathbf{As}^{\prime\mathrm{P}}\\
\dot{\mathbf{r}}^\mathrm{P}=\dot{\mathbf{r}}+\dot{\mathbf{A}}\mathbf{s}^{\prime\mathrm{P}}=\dot{\mathbf{r}}+\dot{\mathbf{A}}\mathbf{A}^\mathrm{T}\mathbf{s}^{\mathrm{P}}\\
\dot{\mathbf{A}}\mathbf{A}^\mathrm{T}+\mathbf{A}\dot{\mathbf{A}}^\mathrm{T}=\mathbf{0},\dot{\mathbf{A}}\mathbf{A}^\mathrm{T}\text{ is skew-symmetric}\\
\widetilde{\omega}=\dot{\mathbf{A}}\mathbf{A}^\mathrm{T},\widetilde{\omega}^\prime=\mathbf{A}^\mathrm{T}\dot{\mathbf{A}},\dot{\mathbf{A}}=\widetilde{\omega}\mathbf{A}
$$

$$
\ddot{\mathbf{r}}^\mathrm{P}=\ddot{\mathbf{r}}+\ddot{\mathbf{A}}\mathbf{s}^{\prime\mathrm{P}}\\
\ddot{\mathbf{A}}=\widetilde{\dot{\omega}}\mathbf{A}+\widetilde{\omega}\dot{\mathbf{A}}=\widetilde{\dot{\omega}}\mathbf{A}+\widetilde{\omega}\widetilde{\omega}\mathbf{A}\\
\ddot{\mathbf{r}}^\mathrm{P}=\ddot{\mathbf{r}}+\widetilde{\dot{\omega}}\mathbf{s}^{\mathrm{P}}+\widetilde{\omega}\widetilde{\omega}\mathbf{s}^{\mathrm{P}}\\
$$

### Infinitesimal Rotation and Displacement

$$
\delta\mathbf{AA}^\mathrm{T}+\mathbf{A}\delta\mathbf{A}^\mathrm{T}=\mathbf{0}\\
\delta\mathbf{AA}^\mathrm{T}\text{ is skew-symmetric}\\
\delta\mathbf{AA}^\mathrm{T}=\delta\tilde{\pi},\delta\mathbf{A}=\delta\tilde{\pi}\mathbf{A}\\
\mathbf{a}=\mathbf{Aa}^\prime,\delta\mathbf{a}=\delta\mathbf{Aa}^\prime=\delta\tilde{\pi}\mathbf{Aa}^\prime=\delta\tilde{\pi}\mathbf{a}
$$

## 2.5 Euler Parameter Orientation Coordinates for a Body in Space

-  $|\mathbf{A}|=1,\exist\mathbf{u}\text{ s.t.}\mathbf{Au}=\mathbf{u}$, the transformation $\mathbf{A}$ leaves the vector $\mathbf{u}$ unchanged (Euler's Theorem)

$$
e_0=\cos\frac{\chi}{2},\mathbf{e}=\sin\frac{\chi}{2}\mathbf{u}\\
\mathbf{A}=(e_0^2-\mathbf{e}^\mathrm{T}\mathbf{e})\mathbf{I}+2\mathbf{ee}^\mathrm{T}+2e_0\tilde{\mathbf{e}}\\
e_0=\pm\frac{1}{2}\sqrt{\tr\mathbf{A}+1},\mathbf{e}=\pm\frac{1}{2\sqrt{\tr\mathbf{A}+1}}\left[\begin{array}{l}
a_{32}-a_{23} \\
a_{13}-a_{31} \\
a_{21}-a_{12}
\end{array}\right]
$$

## 2.6 Euler Parameter Identities and Derivatives

$$
\mathbf{E}(\mathbf{p})=\left[\begin{array}{l} -\mathbf{e} & \tilde{\mathbf{e}}+e_0\mathbf{I} \end{array}\right]\\
\mathbf{G}(\mathbf{p})=\left[\begin{array}{l} -\mathbf{e} & -\tilde{\mathbf{e}}+e_0\mathbf{I} \end{array}\right]\\
\mathbf{A}(\mathbf{p})=\mathbf{E}(\mathbf{p})\mathbf{G}^\mathrm{T}(\mathbf{p})\\
\mathbf{E}(\mathbf{p})\mathbf{p}=\mathbf{G}(\mathbf{p})\mathbf{p}=\mathbf{0}\\
\mathbf{E}(\mathbf{p})\mathbf{E}^\mathrm{T}(\mathbf{p})=\mathbf{G}(\mathbf{p})\mathbf{G}^\mathrm{T}(\mathbf{p})=\mathbf{p}^\mathrm{T}\mathbf{pI}\\
\mathbf{E}^\mathrm{T}(\mathbf{p})\mathbf{E}(\mathbf{p})=\mathbf{G}^\mathrm{T}(\mathbf{p})\mathbf{G}(\mathbf{p})=\mathbf{p}^\mathrm{T}\mathbf{pI}_4-\mathbf{p}\mathbf{p}^\mathrm{T}\\
\mathbf{AA}^\mathrm{T}=\mathbf{A}^\mathrm{T}\mathbf{A}=\left(\mathbf{p}^\mathrm{T}\mathbf{p}\right)^2\mathbf{I}\\
\mathbf{E}(\mathbf{p}_i)\mathbf{p}_j=-\mathbf{E}(\mathbf{p}_j)\mathbf{p}_i,\mathbf{G}(\mathbf{p}_i)\mathbf{p}_j=-\mathbf{G}(\mathbf{p}_j)\mathbf{p}_i\\
\mathbf{E}(\mathbf{p}_i)\mathbf{G}^\mathrm{T}(\mathbf{p}_j)=\mathbf{E}(\mathbf{p}_j)\mathbf{G}^\mathrm{T}(\mathbf{p}_i),\mathbf{G}(\mathbf{p}_i)\mathbf{E}^\mathrm{T}(\mathbf{p}_j)=\mathbf{G}(\mathbf{p}_j)\mathbf{E}^\mathrm{T}(\mathbf{p}_i)
$$

$$
\text{Define } \mathbf{R}(\mathbf{a}) =\left[\begin{array}{cc}
0 & -\mathbf{a}^{\mathrm{T}} \\
\mathbf{a} & \tilde{\mathbf{a}}
\end{array}\right],
\mathbf{T}(\mathbf{a}) =\left[\begin{array}{cc}
0 & -\mathbf{a}^{\mathrm{T}} \\
\mathbf{a} & -\tilde{\mathbf{a}}
\end{array}\right]\\
\mathbf{R}(\mathbf{a})\mathbf{p}=\mathbf{E}^\mathrm{T}(\mathbf{p})\mathbf{a},\mathbf{T}(\mathbf{a})\mathbf{p}=\mathbf{G}^\mathrm{T}(\mathbf{p})\mathbf{a}
$$

### Euler Parameter Derivatives

$$
\mathbf{B}(\mathbf{p},\mathbf{a}^\prime)=\left(\mathbf{A}(\mathbf{p})\mathbf{a}^\prime\right)_\mathbf{p}=2\mathbf{E}(\mathbf{p})\mathbf{T}(\mathbf{a}^\prime)\\
\mathbf{B}(\mathbf{p}_i,\mathbf{a}^\prime)\mathbf{p}_j=\mathbf{B}(\mathbf{p}_j,\mathbf{a}^\prime)\mathbf{p}_i\\
\left(\mathbf{B}(\mathbf{p}_i,\mathbf{a}^\prime)\mathbf{p}_j\right)_{\mathbf{p}_i}=\left(\mathbf{B}(\mathbf{p}_j,\mathbf{a}^\prime)\mathbf{p}_i\right)_{\mathbf{p}_i}=\mathbf{B}(\mathbf{p}_j,\mathbf{a}^\prime)\\
\mathbf{C}(\mathbf{p},\mathbf{a})=\left(\mathbf{A}^\mathrm{T}(\mathbf{p})\mathbf{a}\right)_\mathbf{p}=2\mathbf{G}(\mathbf{p})\mathbf{R}(\mathbf{a})\\
\mathbf{C}(\mathbf{p}_i,\mathbf{a})\mathbf{p}_j=\mathbf{C}(\mathbf{p}_j,\mathbf{a})\mathbf{p}_i\\
\left(\mathbf{C}(\mathbf{p}_i,\mathbf{a})\mathbf{p}_j\right)_{\mathbf{p}_i}=\left(\mathbf{C}(\mathbf{p}_j,\mathbf{a})\mathbf{p}_i\right)_{\mathbf{p}_i}=\mathbf{C}(\mathbf{p}_j,\mathbf{a})\\
$$

$$
\mathbf{B}^\mathrm{T}(\mathbf{p},\mathbf{a}^\prime)\mathbf{b}=\mathbf{K}(\mathbf{a}^\prime,\mathbf{b})\mathbf{p}\\
\mathbf{K}(\mathbf{a}^\prime,\mathbf{b})=2\left[\begin{array}{cc}
\mathbf{a}^{\prime \mathrm{T}} \mathbf{b} & \mathbf{a}^{\prime \mathrm{T}} \tilde{\mathbf{b}} \\
\tilde{\mathbf{a}}^{\prime} \mathbf{b} & \mathbf{a}^{\prime} \mathbf{b}^{\mathrm{T}}+\mathbf{b a}^{\prime \mathrm{T}}-\mathbf{a}^{\prime \mathrm{T}} \mathbf{b I}
\end{array}\right]\text{ is symmetric}\\
\left(\mathbf{B}^\mathrm{T}(\mathbf{p},\mathbf{a}^\prime)\gamma\right)_\mathbf{p}=\left(\mathbf{K}(\mathbf{a}^\prime,\gamma)\mathbf{p}\right)_\mathbf{p}=\mathbf{K}(\mathbf{a}^\prime,\gamma)\\
\mathbf{C}^\mathrm{T}(\mathbf{p},\mathbf{a})\mathbf{b}=\mathbf{L}(\mathbf{a},\mathbf{b})\mathbf{p}\\
\mathbf{L}(\mathbf{a},\mathbf{b})=2\left[\begin{array}{cc}
\mathbf{a}^{\mathrm{T}} \mathbf{b} & -\mathbf{a}^\mathrm{T} \tilde{\mathbf{b}} \\
-\tilde{\mathbf{a}} \mathbf{b} & \mathbf{a} \mathbf{b}^{\mathrm{T}}+\mathbf{b a}^\mathrm{T}-\mathbf{a}^\mathrm{T} \mathbf{b I}
\end{array}\right]\text{ is symmetric}\\
\left(\mathbf{C}^\mathrm{T}(\mathbf{p},\mathbf{a})\mathbf{b}\right)_\mathbf{p}=\left(\mathbf{L}(\mathbf{a},\mathbf{b})\mathbf{p}\right)_\mathbf{p}=\mathbf{L}(\mathbf{a},\mathbf{b})\\
$$

