# M2

$$
\left\{\begin{array}{l}
q_{1}=l_{3} s_{\beta}+P_{z}-a_{1} \\
q_{2}=-l_{4} c_{\beta} s_{\alpha}+h_{1} c_{\beta} c_{\alpha}+P_{z}-a_{2} \\
q_{3}=-l_{3} s_{\beta}+P_{z}-a_{3} \\
q_{4}=l_{4} c_{\beta} s_{\alpha}+h_{1} c_{\beta} c_{\alpha}+P_{z}-a_{4}
\end{array}\right.\\
\left\{\begin{array}{l}
a_{1}=\sqrt{l^{2}-\left(P_{x}-l_{3} c_{\beta}+l_{1}\right)^{2}} \\
a_{2}=\sqrt{l^{2}-\left(-2 l_{4} s_{\beta} s_{\alpha}\right)^{2}-\left(l_{2}-l_{4} c_{\alpha}-h_{1} s_{\alpha}\right)^{2}} \\
a_{3}=\sqrt{l^{2}-\left(P_{x}+l_{3} c_{\beta}-l_{1}\right)^{2}} \\
a_{4}=\sqrt{l^{2}-\left(l_{4} c_{\alpha}-h_{1} s_{\alpha}-l_{2}\right)^{2}}
\end{array}\right.\\
P_x=-l_4s_\beta s_\alpha-h_1s_\beta c_\alpha
$$

$$
\left\{\begin{array}{l}
q_{1}=l_{3} s_{\beta}+P_{z}-\sqrt{l^{2}-\left(-l_4s_\beta s_\alpha-h_1s_\beta c_\alpha-l_{3} c_{\beta}+l_{1}\right)^{2}} \\
q_{2}=-l_{4} c_{\beta} s_{\alpha}+h_{1} c_{\beta} c_{\alpha}+P_{z}-\sqrt{l^{2}-\left(-2 l_{4} s_{\beta} s_{\alpha}\right)^{2}-\left(l_{2}-l_{4} c_{\alpha}-h_{1} s_{\alpha}\right)^{2}} \\
q_{3}=-l_{3} s_{\beta}+P_{z}-\sqrt{l^{2}-\left(-l_4s_\beta s_\alpha-h_1s_\beta c_\alpha+l_{3} c_{\beta}-l_{1}\right)^{2}} \\
q_{4}=l_{4} c_{\beta} s_{\alpha}+h_{1} c_{\beta} c_{\alpha}+P_{z}-\sqrt{l^{2}-\left(l_{4} c_{\alpha}-h_{1} s_{\alpha}-l_{2}\right)^{2}}
\end{array}\right.\\
$$

